backend/Stackingproof.v
@@ -2411,9 +2411,9 @@ Proof.
       rewrite <- sep_assoc. repeat (apply conj; auto).
       * tinv.
       * intros b ofs Hofs (b0 & delta & Hb & Hp). eapply H11; eauto.
-      * intros ? ?. cbn. contradiction.
+      * red. intros. red in H1. red in H2. simpl in H1. simpl in H2. admit.
     + inv H0. auto.
-Qed.
+Admitted.
 
 Lemma transf_final_states:
   forall w st1 st2 r1, wt_state prog se st1 -> match_states w st1 st2 -> Linear.final_state st1 r1 ->
@@ -2477,14 +2477,15 @@ Proof.
         eapply stack_contents_support; eauto. apply SEP.
       * intros r. cbn. destruct in_dec; eauto.
         destruct is_callee_save eqn:Hr; eauto.
-      * eapply stack_contents_change_meminj; eauto.
+      * admit.
+        (*eapply stack_contents_change_meminj; eauto.
         rewrite sep_comm, sep_assoc in SEP |- *.
         eapply minjection_incr; eauto.
         rewrite sep_comm, sep_assoc in SEP |- *.
         eapply globalenv_inject_incr; eauto. destruct H12.
-        eapply Mem.unchanged_on_support; eauto.
+        eapply Mem.unchanged_on_support; eauto. *)
       * inversion Hm'. eauto.
-Qed.
+Admitted.
 
 Lemma wt_prog:
   forall i fd, In (i, Gfun fd) prog.(prog_defs) -> wt_fundef fd.
